@prefix : <http://www.semanticweb.org/antoinelouis/ontologies/2019/4/olympic-games#> .
@prefix owl: <http://www.w3.org/2002/07/owl#> .
@prefix rdf: <http://www.w3.org/1999/02/22-rdf-syntax-ns#> .
@prefix xml: <http://www.w3.org/XML/1998/namespace> .
@prefix xsd: <http://www.w3.org/2001/XMLSchema#> .
@prefix rdfs: <http://www.w3.org/2000/01/rdf-schema#> .
@base <http://www.semanticweb.org/antoinelouis/ontologies/2019/4/olympic-games> .

<http://www.semanticweb.org/antoinelouis/ontologies/2019/4/olympic-games> rdf:type owl:Ontology .

#################################################################
#    Object Properties
#################################################################

###  http://www.semanticweb.org/antoinelouis/ontologies/2019/4/olympic-games#hasAwardedFirstPlace
:hasAwardedFirstPlace rdf:type owl:ObjectProperty ;
                      rdfs:subPropertyOf owl:topObjectProperty ;
                      owl:inverseOf :isFirstPlaceWinnerOf ;
                      rdfs:comment "A SportCompetition has awarded an Athlete the title of first place." .


###  http://www.semanticweb.org/antoinelouis/ontologies/2019/4/olympic-games#hasAwardedSecondPlace
:hasAwardedSecondPlace rdf:type owl:ObjectProperty ;
                       rdfs:subPropertyOf owl:topObjectProperty ;
                       owl:inverseOf :isSecondPlaceWinnerOf ;
                       rdfs:comment "A SportCompetition has awarded an Athlete the title of first place." .


###  http://www.semanticweb.org/antoinelouis/ontologies/2019/4/olympic-games#hasAwardedThirdPlace
:hasAwardedThirdPlace rdf:type owl:ObjectProperty ;
                      rdfs:subPropertyOf owl:topObjectProperty ;
                      owl:inverseOf :isThirdPlaceWinnerOf ;
                      rdfs:comment "A SportCompetition has awarded an Athlete the title of third place." .


###  http://www.semanticweb.org/antoinelouis/ontologies/2019/4/olympic-games#hasCompetitor
:hasCompetitor rdf:type owl:ObjectProperty ;
               owl:inverseOf :isCompetitorIn ;
               rdfs:comment "A SportCompetition has Athletes that compete in it." .


###  http://www.semanticweb.org/antoinelouis/ontologies/2019/4/olympic-games#hasHost
:hasHost rdf:type owl:ObjectProperty ;
         owl:inverseOf :isHostOf ;
         rdf:type owl:TransitiveProperty ;
         rdfs:comment "A SportCompetition is hosted by a kind of OlympicGame" .


###  http://www.semanticweb.org/antoinelouis/ontologies/2019/4/olympic-games#hasRound
:hasRound rdf:type owl:ObjectProperty ;
          owl:inverseOf :isRoundIn ;
          rdfs:domain :MultiRoundCompetition ;
          rdfs:range :Round ;
          rdfs:comment "A MultiRoundCompetition has Rounds that are played as part of it" .


###  http://www.semanticweb.org/antoinelouis/ontologies/2019/4/olympic-games#hasSport
:hasSport rdf:type owl:ObjectProperty ;
          rdfs:comment "A SportCompetition has a Sport that is played in that competition" .


###  http://www.semanticweb.org/antoinelouis/ontologies/2019/4/olympic-games#hasStage
:hasStage rdf:type owl:ObjectProperty ;
          owl:inverseOf :isStageIn ;
          rdfs:domain :MultiStageCompetition ;
          rdfs:range :Stage ;
          rdfs:comment "A MultiStageCompetition has instances of Stage as competition" .


###  http://www.semanticweb.org/antoinelouis/ontologies/2019/4/olympic-games#hasUnitCompetition
:hasUnitCompetition rdf:type owl:ObjectProperty ;
                    owl:inverseOf :isUnitCompetitionOf ;
                    rdfs:comment "A Round or a Stage has UnitCompetitions as part of it." .


###  http://www.semanticweb.org/antoinelouis/ontologies/2019/4/olympic-games#isCompetitorIn
:isCompetitorIn rdf:type owl:ObjectProperty ;
                rdfs:domain [ rdf:type owl:Restriction ;
                              owl:onProperty :isCompetitorIn ;
                              owl:someValuesFrom :Athlete
                            ] ;
                rdfs:range [ rdf:type owl:Restriction ;
                             owl:onProperty :isCompetitorIn ;
                             owl:someValuesFrom :SportCompetition
                           ] ;
                rdfs:comment "An Athlete competes in a kind of SportCompetition" .


###  http://www.semanticweb.org/antoinelouis/ontologies/2019/4/olympic-games#isFirstPlaceWinnerOf
:isFirstPlaceWinnerOf rdf:type owl:ObjectProperty ;
                      rdfs:comment "An Athlete wins first place in a SportCompetition." .


###  http://www.semanticweb.org/antoinelouis/ontologies/2019/4/olympic-games#isHostOf
:isHostOf rdf:type owl:ObjectProperty ,
                   owl:TransitiveProperty ;
          rdfs:domain :OlympicGame ;
          rdfs:range :SportCompetition ;
          rdfs:comment "An OlympicGame is host to a kind of SportCompetition" .


###  http://www.semanticweb.org/antoinelouis/ontologies/2019/4/olympic-games#isPlayedBy
:isPlayedBy rdf:type owl:ObjectProperty ;
            owl:inverseOf :plays ;
            rdfs:comment "A Sport is played by an Athlete" .


###  http://www.semanticweb.org/antoinelouis/ontologies/2019/4/olympic-games#isRoundIn
:isRoundIn rdf:type owl:ObjectProperty ;
           rdfs:comment "A round is part of a MultiRoundCompetition" .


###  http://www.semanticweb.org/antoinelouis/ontologies/2019/4/olympic-games#isSecondPlaceWinnerOf
:isSecondPlaceWinnerOf rdf:type owl:ObjectProperty ;
                       rdfs:comment "An Athlete wins second place in a SportCompetition." .


###  http://www.semanticweb.org/antoinelouis/ontologies/2019/4/olympic-games#isStageIn
:isStageIn rdf:type owl:ObjectProperty ;
           rdfs:comment "A stage is part of a MultiStageCompetition" .


###  http://www.semanticweb.org/antoinelouis/ontologies/2019/4/olympic-games#isThirdPlaceWinnerOf
:isThirdPlaceWinnerOf rdf:type owl:ObjectProperty ;
                      rdfs:subPropertyOf owl:topObjectProperty ;
                      rdfs:comment "An Athlete wins third place in a SportCompetition." .


###  http://www.semanticweb.org/antoinelouis/ontologies/2019/4/olympic-games#isUnitCompetitionOf
:isUnitCompetitionOf rdf:type owl:ObjectProperty ;
                     rdfs:comment "A UnitCompetition belongs to a Stage, a Round or is by itself." .


###  http://www.semanticweb.org/antoinelouis/ontologies/2019/4/olympic-games#plays
:plays rdf:type owl:ObjectProperty ;
       rdfs:domain :Athlete ;
       rdfs:range :Sport ;
       rdfs:comment "An Athlete plays a Sport" .


#################################################################
#    Data properties
#################################################################

###  http://www.semanticweb.org/antoinelouis/ontologies/2019/4/olympic-games#hasAge
:hasAge rdf:type owl:DatatypeProperty ;
        rdfs:domain :Athlete ;
        rdfs:range xsd:int ;
        rdfs:comment """Age of a person in years.
Example: 32""" .


###  http://www.semanticweb.org/antoinelouis/ontologies/2019/4/olympic-games#hasEquipment
:hasEquipment rdf:type owl:DatatypeProperty ;
              rdfs:domain :Sport ;
              rdfs:range xsd:string .


###  http://www.semanticweb.org/antoinelouis/ontologies/2019/4/olympic-games#hasFirstName
:hasFirstName rdf:type owl:DatatypeProperty ;
              rdfs:domain :Athlete ;
              rdfs:range xsd:string ;
              rdfs:comment "Firstname of a person." .


###  http://www.semanticweb.org/antoinelouis/ontologies/2019/4/olympic-games#hasGender
:hasGender rdf:type owl:DatatypeProperty ;
           rdfs:domain :Athlete ;
           rdfs:range xsd:string ;
           rdfs:comment """Gender of a person.
Example: \"male\" or \"female\"""" .


###  http://www.semanticweb.org/antoinelouis/ontologies/2019/4/olympic-games#hasHeight
:hasHeight rdf:type owl:DatatypeProperty ;
           rdfs:domain :Athlete ;
           rdfs:range xsd:int ;
           rdfs:comment """Height of a person in cm.
Example: 190""" .


###  http://www.semanticweb.org/antoinelouis/ontologies/2019/4/olympic-games#hasLastName
:hasLastName rdf:type owl:DatatypeProperty ;
             rdfs:domain :Athlete ;
             rdfs:range xsd:string ;
             rdfs:comment "Last name of a person." .


###  http://www.semanticweb.org/antoinelouis/ontologies/2019/4/olympic-games#hasWeight
:hasWeight rdf:type owl:DatatypeProperty ;
           rdfs:domain :Athlete ;
           rdfs:range xsd:int ;
           rdfs:comment """Weight of a person in kg.
Example: 85""" .


###  http://www.semanticweb.org/antoinelouis/ontologies/2019/4/olympic-games#playsSport
:playsSport rdf:type owl:DatatypeProperty ;
            rdfs:domain :Sport ;
            rdfs:range xsd:string ;
            rdfs:comment """Name of the sport.
Example: \"Tennis\"""" .


#################################################################
#    Classes
#################################################################

###  http://www.semanticweb.org/antoinelouis/ontologies/2019/4/olympic-games#Athlete
:Athlete rdf:type owl:Class ;
         rdfs:subClassOf [ rdf:type owl:Restriction ;
                           owl:onProperty :plays ;
                           owl:someValuesFrom :Sport
                         ] ;
         rdfs:comment """An athlete is a person who practices some sport(s).
Example: the tennis player Rafael Nadal.""" .


###  http://www.semanticweb.org/antoinelouis/ontologies/2019/4/olympic-games#AthleticsSport
:AthleticsSport rdf:type owl:Class ;
                rdfs:subClassOf :Sport ;
                rdfs:comment """Athletics sport is the sport of competing in track and field events, including running races and various competitions in jumping and throwing.
Example: 100M, 400M, Hammer Throw, High Jump.""" .


###  http://www.semanticweb.org/antoinelouis/ontologies/2019/4/olympic-games#BallSport
:BallSport rdf:type owl:Class ;
           rdfs:subClassOf :Sport ;
           rdfs:comment """A ball sport is any form of sport which features a ball as part of play.
Example: football, cricket, baseball, basketball.""" .


###  http://www.semanticweb.org/antoinelouis/ontologies/2019/4/olympic-games#CombatSport
:CombatSport rdf:type owl:Class ;
             rdfs:subClassOf :Sport ;
             rdfs:comment """A combat sport is a competitive contact sport that usually involves one-on-one combat.
Example:  boxing, wrestling, fencing, savate.""" .


###  http://www.semanticweb.org/antoinelouis/ontologies/2019/4/olympic-games#MultiDisciplineCompetition
:MultiDisciplineCompetition rdf:type owl:Class ;
                            rdfs:subClassOf :SportCompetition ,
                                            [ rdf:type owl:Restriction ;
                                              owl:onProperty :hasSport ;
                                              owl:minQualifiedCardinality "2"^^xsd:nonNegativeInteger ;
                                              owl:onClass :Sport
                                            ] ;
                            rdfs:comment """A competition that incorporates a number of different sports, that is at least 2.
Example: Athletics competition.""" .


###  http://www.semanticweb.org/antoinelouis/ontologies/2019/4/olympic-games#MultiRoundCompetition
:MultiRoundCompetition rdf:type owl:Class ;
                       rdfs:subClassOf :SportCompetition ,
                                       [ rdf:type owl:Restriction ;
                                         owl:onProperty :hasRound ;
                                         owl:minQualifiedCardinality "2"^^xsd:nonNegativeInteger ;
                                         owl:onClass :Round
                                       ] ;
                       rdfs:comment """A multi-round competition is a competition organised as a sequence of rounds where the winner advances and the loser gets eliminated.
Example: the Wimbledon tennis tournament.""" .


###  http://www.semanticweb.org/antoinelouis/ontologies/2019/4/olympic-games#MultiSport
:MultiSport rdf:type owl:Class ;
            rdfs:subClassOf :Sport ;
            rdfs:comment """A multisport is a sport in which athletes compete in multiple athletic disciplines.
Example: Triathlon (running, swimming, cycling)""" .


###  http://www.semanticweb.org/antoinelouis/ontologies/2019/4/olympic-games#MultiStageCompetition
:MultiStageCompetition rdf:type owl:Class ;
                       rdfs:subClassOf :SportCompetition ,
                                       [ rdf:type owl:Restriction ;
                                         owl:onProperty :hasStage ;
                                         owl:minQualifiedCardinality "2"^^xsd:nonNegativeInteger ;
                                         owl:onClass :Stage
                                       ] ;
                       rdfs:comment """A Multi-stage Competition is a competition that is organised as a set of stages.
Example: the Football World Cup.""" .


###  http://www.semanticweb.org/antoinelouis/ontologies/2019/4/olympic-games#OlympicGame
:OlympicGame rdf:type owl:Class ;
             rdfs:subClassOf [ rdf:type owl:Restriction ;
                               owl:onProperty :isHostOf ;
                               owl:someValuesFrom :SportCompetition
                             ] ;
             rdfs:comment "The Olympic Games are an international sporting event in which thousands of athletes from around the world participate in a variety of competitions." .


###  http://www.semanticweb.org/antoinelouis/ontologies/2019/4/olympic-games#Round
:Round rdf:type owl:Class ;
       rdfs:subClassOf [ rdf:type owl:Restriction ;
                         owl:onProperty :hasUnitCompetition ;
                         owl:someValuesFrom :UnitCompetition
                       ] ,
                       [ rdf:type owl:Restriction ;
                         owl:onProperty :isRoundIn ;
                         owl:someValuesFrom :MultiRoundCompetition
                       ] ;
       rdfs:comment """A round is one or more competitions that is part of a Multi-Round Competition.
Example: first round of Wimbledon.""" .


###  http://www.semanticweb.org/antoinelouis/ontologies/2019/4/olympic-games#Sport
:Sport rdf:type owl:Class ;
       rdfs:comment "A sport is a phyisical activity in which an individual or team competes against another or others for entertainment." .


###  http://www.semanticweb.org/antoinelouis/ontologies/2019/4/olympic-games#SportCompetition
:SportCompetition rdf:type owl:Class ;
                  rdfs:subClassOf [ rdf:type owl:Restriction ;
                                    owl:onProperty :hasCompetitor ;
                                    owl:someValuesFrom :Athlete
                                  ] ,
                                  [ rdf:type owl:Restriction ;
                                    owl:onProperty :hasHost ;
                                    owl:someValuesFrom :OlympicGame
                                  ] ,
                                  [ rdf:type owl:Restriction ;
                                    owl:onProperty :hasSport ;
                                    owl:someValuesFrom :Sport
                                  ] ;
                  rdfs:comment "A sport competition is a competitive sporting event." .


###  http://www.semanticweb.org/antoinelouis/ontologies/2019/4/olympic-games#Stage
:Stage rdf:type owl:Class ;
       rdfs:subClassOf [ rdf:type owl:Restriction ;
                         owl:onProperty :hasUnitCompetition ;
                         owl:someValuesFrom :UnitCompetition
                       ] ,
                       [ rdf:type owl:Restriction ;
                         owl:onProperty :isStageIn ;
                         owl:someValuesFrom :MultiStageCompetition
                       ] ;
       rdfs:comment """A stage is one or more competitions part of a MultiStageCompetition where the N best teams/players only advance in the competition.
Example: pooling stage of Football World Cup""" .


###  http://www.semanticweb.org/antoinelouis/ontologies/2019/4/olympic-games#SummerGame
:SummerGame rdf:type owl:Class ;
            rdfs:subClassOf :OlympicGame ;
            owl:disjointWith :WinterGame ;
            rdfs:comment """Summer Game is a kind of Olympic Game consisting only of 
summer sports.""" .


###  http://www.semanticweb.org/antoinelouis/ontologies/2019/4/olympic-games#UnitCompetition
:UnitCompetition rdf:type owl:Class ;
                 rdfs:subClassOf :SportCompetition ;
                 rdfs:comment """A unit competition is the unit of competition defined by a competition discipline rules. 
Example: a tennis match or a 100m race.""" .


###  http://www.semanticweb.org/antoinelouis/ontologies/2019/4/olympic-games#WaterSport
:WaterSport rdf:type owl:Class ;
            rdfs:subClassOf :Sport ;
            rdfs:comment """A water sport is a sport happening in or involving water.
Example: kanoe, sailing, diving""" .


###  http://www.semanticweb.org/antoinelouis/ontologies/2019/4/olympic-games#WinterGame
:WinterGame rdf:type owl:Class ;
            rdfs:subClassOf :OlympicGame ;
            rdfs:comment "Winter Game is a kind of Olympic Game consisting only of winter sports." .


#################################################################
#    Individuals
#################################################################

###  http://www.semanticweb.org/antoinelouis/ontologies/2019/4/olympic-games#Biathlon
:Biathlon rdf:type owl:NamedIndividual ,
                   :MultiSport .


###  http://www.semanticweb.org/antoinelouis/ontologies/2019/4/olympic-games#Bolt
:Bolt rdf:type owl:NamedIndividual ,
               :Athlete ;
      :hasAge "32"^^xsd:int ;
      :hasFirstName "Usain"^^xsd:string ;
      :hasGender "Male"^^xsd:string ;
      :hasHeight "195"^^xsd:int ;
      :hasLastName "Bolt"^^xsd:string ;
      :hasWeight "94"^^xsd:int .


###  http://www.semanticweb.org/antoinelouis/ontologies/2019/4/olympic-games#Boxing
:Boxing rdf:type owl:NamedIndividual ,
                 :CombatSport .


###  http://www.semanticweb.org/antoinelouis/ontologies/2019/4/olympic-games#Diving
:Diving rdf:type owl:NamedIndividual ,
                 :WaterSport .


###  http://www.semanticweb.org/antoinelouis/ontologies/2019/4/olympic-games#Football
:Football rdf:type owl:NamedIndividual ,
                   :BallSport .


###  http://www.semanticweb.org/antoinelouis/ontologies/2019/4/olympic-games#HammerThrow
:HammerThrow rdf:type owl:NamedIndividual ,
                      :AthleticsSport .


###  http://www.semanticweb.org/antoinelouis/ontologies/2019/4/olympic-games#HighJump
:HighJump rdf:type owl:NamedIndividual ,
                   :AthleticsSport .


###  http://www.semanticweb.org/antoinelouis/ontologies/2019/4/olympic-games#Judo
:Judo rdf:type owl:NamedIndividual ,
               :CombatSport .


###  http://www.semanticweb.org/antoinelouis/ontologies/2019/4/olympic-games#Swimming
:Swimming rdf:type owl:NamedIndividual ,
                   :WaterSport .


###  http://www.semanticweb.org/antoinelouis/ontologies/2019/4/olympic-games#Taekwondo
:Taekwondo rdf:type owl:NamedIndividual ,
                    :CombatSport .


###  http://www.semanticweb.org/antoinelouis/ontologies/2019/4/olympic-games#Tennis
:Tennis rdf:type owl:NamedIndividual ,
                 :BallSport ;
        :hasEquipment "Racket"^^xsd:string ;
        :playsSport "Tennis"^^xsd:string .


###  http://www.semanticweb.org/antoinelouis/ontologies/2019/4/olympic-games#Triathlon
:Triathlon rdf:type owl:NamedIndividual ,
                    :MultiSport .


###  http://www.semanticweb.org/antoinelouis/ontologies/2019/4/olympic-games#Volleyball
:Volleyball rdf:type owl:NamedIndividual ,
                     :BallSport .


###  http://www.semanticweb.org/antoinelouis/ontologies/2019/4/olympic-games#Waterpolo
:Waterpolo rdf:type owl:NamedIndividual ,
                    :WaterSport .


###  http://www.semanticweb.org/antoinelouis/ontologies/2019/4/olympic-games#100M
<http://www.semanticweb.org/antoinelouis/ontologies/2019/4/olympic-games#100M> rdf:type owl:NamedIndividual ,
                                                                                        :AthleticsSport .


#################################################################
#    General axioms
#################################################################

[ rdf:type owl:AllDisjointClasses ;
  owl:members ( :Athlete
                :OlympicGame
                :Round
                :Sport
                :SportCompetition
                :Stage
              )
] .


[ rdf:type owl:AllDisjointClasses ;
  owl:members ( :MultiDisciplineCompetition
                :MultiRoundCompetition
                :MultiStageCompetition
                :UnitCompetition
              )
] .


[ rdf:type owl:AllDifferent ;
  owl:distinctMembers ( :Biathlon
                        :Bolt
                        :Boxing
                        :Diving
                        :Football
                        :HammerThrow
                        :HighJump
                        :Judo
                        :Swimming
                        :Taekwondo
                        :Tennis
                        :Triathlon
                        :Volleyball
                        :Waterpolo
                        <http://www.semanticweb.org/antoinelouis/ontologies/2019/4/olympic-games#100M>
                      )
] .


###  Generated by the OWL API (version 4.5.9.2019-02-01T07:24:44Z) https://github.com/owlcs/owlapi
